src/proof/controllers/statefulset/name.v
@@ -1,14 +1,16 @@
 From New.proof Require Import prelude empty_ffi.
 From New.proof.string Require Export prefix_suffix.
 From New.proof Require Export pure_objects.
+From New.proof Require Export external_wp.
 
-Definition desired_pod_name (sts : StatefulSetV.t) (ordinal : nat) : go_string :=
-  sts.(StatefulSetV.ObjectMeta').(ObjectMetaV.Name') ++ "-"%go ++ decimal_string ordinal.
+Definition desired_pod_name (set_name : go_string) (ordinal : nat) : go_string :=
+  set_name ++ "-"%go ++ decimal_string ordinal.
 
-Definition desired_pod_key (sts : StatefulSetV.t) (ordinal : nat) : KKey.t := {|
+Definition desired_pod_key sts ordinal : KKey.t := {|
   KKey.Kind' := PodV.kind;
   KKey.Namespace' := sts.(StatefulSetV.ObjectMeta').(ObjectMetaV.Namespace');
-  KKey.Name' := desired_pod_name sts ordinal;
+  KKey.Name' := desired_pod_name
+    sts.(StatefulSetV.ObjectMeta').(ObjectMetaV.Name') ordinal;
 |}.
 
 Definition statefulset_replicas (sts : StatefulSetV.t) : nat :=
@@ -25,15 +27,14 @@ Definition pvc_claim_template_names (sts : StatefulSetV.t) : list go_string :=
     claim_template.(PersistentVolumeClaimV.ObjectMeta').(ObjectMetaV.Name'))
   <$> sts.(StatefulSetV.Spec').(StatefulSetSpecV.VolumeClaimTemplates').
 
-Definition desired_pvc_name sts claim_template_name ordinal : go_string :=
-  claim_template_name ++ "-"%go ++
-  sts.(StatefulSetV.ObjectMeta').(ObjectMetaV.Name') ++ "-"%go ++
-  decimal_string ordinal.
+Definition desired_pvc_name set_name claim_template_name ordinal : go_string :=
+  claim_template_name ++ "-"%go ++ set_name ++ "-"%go ++ decimal_string ordinal.
 
 Definition desired_pvc_key sts claim_template_name ordinal : KKey.t := {|
   KKey.Kind' := PersistentVolumeClaimV.kind;
   KKey.Namespace' := sts.(StatefulSetV.ObjectMeta').(ObjectMetaV.Namespace');
-  KKey.Name' := desired_pvc_name sts claim_template_name ordinal;
+  KKey.Name' := desired_pvc_name
+    sts.(StatefulSetV.ObjectMeta').(ObjectMetaV.Name') claim_template_name ordinal;
 |}.
 
 Definition desired_pvc_key_candidates sts : list KKey.t :=
@@ -59,30 +60,67 @@ Definition pod_key_is_desired (sts : StatefulSetV.t) (key : KKey.t) : Prop :=
     Decision (pod_key_is_desired sts key).
 Proof. unfold pod_key_is_desired. apply _. Defined.
 
-Definition pod_has_member_name (sts : StatefulSetV.t) (pod : PodV.t) : Prop :=
-  ∃ ordinal,
-    pod.(PodV.ObjectMeta').(ObjectMetaV.Name') = desired_pod_name sts ordinal.
+Definition pod_has_member_name (set_name pod_name : go_string) : Prop :=
+  ∃ ordinal, pod_name = desired_pod_name set_name ordinal.
 
 Definition pod_has_member_key (sts : StatefulSetV.t) (pod : PodV.t) : Prop :=
   ∃ ordinal, PodV.key pod = desired_pod_key sts ordinal.
 
-Definition member_name_prefix (sts : StatefulSetV.t) : go_string :=
-  sts.(StatefulSetV.ObjectMeta').(ObjectMetaV.Name') ++ "-"%go.
+Lemma desired_pod_name_inj set_name ordinal1 ordinal2 :
+  desired_pod_name set_name ordinal1 = desired_pod_name set_name ordinal2 →
+  ordinal1 = ordinal2.
+Proof.
+  unfold desired_pod_name.
+  intros Hname.
+  apply app_inv_head in Hname.
+  inversion Hname as [Hdecimal].
+  by apply decimal_string_inj in Hdecimal.
+Qed.
 
-Definition parse_member_name (sts : StatefulSetV.t) (pod : PodV.t) : option nat :=
-  match New.proof.string.prefix_suffix.strip_prefix (member_name_prefix sts)
-      (pod.(PodV.ObjectMeta').(ObjectMetaV.Name')) with
+Lemma desired_pod_name_last_dash_decomp pod_name parent suffix set_name ordinal :
+  pod_name = parent ++ [byte_dash] ++ suffix →
+  byte_dash ∉ suffix →
+  pod_name = desired_pod_name set_name ordinal →
+  parent = set_name ∧ suffix = decimal_string ordinal.
+Proof.
+  intros Hdecomp Hsuffix_no_dash Hdesired.
+  rewrite Hdesired in Hdecomp.
+  unfold desired_pod_name in Hdecomp.
+  change "-"%go with [byte_dash] in Hdecomp.
+  eapply app_last_sep_inj in Hdecomp.
+  - destruct Hdecomp as [Hparent Hsuffix].
+    split; symmetry; done.
+  - apply decimal_string_dash_free.
+  - by apply dash_free_of_not_elem.
+Qed.
+
+Lemma desired_pod_name_has_dash set_name ordinal :
+  byte_dash ∈ desired_pod_name set_name ordinal.
+Proof.
+  unfold desired_pod_name.
+  change "-"%go with [byte_dash].
+  rewrite elem_of_app. right.
+  rewrite elem_of_app. left.
+  rewrite elem_of_cons. by left.
+Qed.
+
+Definition member_name_prefix (set_name : go_string) : go_string :=
+  set_name ++ "-"%go.
+
+Definition parse_member_name (set_name pod_name : go_string) : option nat :=
+  match New.proof.string.prefix_suffix.strip_prefix (member_name_prefix set_name)
+      pod_name with
   | Some suffix => parse_canonical_decimal_string suffix
   | None => None
   end.
 
-Lemma parse_member_name_sound sts pod ordinal :
-  parse_member_name sts pod = Some ordinal →
-  pod.(PodV.ObjectMeta').(ObjectMetaV.Name') = desired_pod_name sts ordinal.
+Lemma parse_member_name_sound set_name pod_name ordinal :
+  parse_member_name set_name pod_name = Some ordinal →
+  pod_name = desired_pod_name set_name ordinal.
 Proof.
   unfold parse_member_name.
-  destruct (New.proof.string.prefix_suffix.strip_prefix (member_name_prefix sts)
-    (pod.(PodV.ObjectMeta').(ObjectMetaV.Name'))) as [suffix|] eqn:Hstrip; [|done].
+  destruct (New.proof.string.prefix_suffix.strip_prefix (member_name_prefix set_name)
+    pod_name) as [suffix|] eqn:Hstrip; [|done].
   intros Hparse.
   apply parse_canonical_decimal_string_sound in Hparse.
   apply New.proof.string.prefix_suffix.strip_prefix_correct in Hstrip.
@@ -92,9 +130,9 @@ Proof.
   by rewrite List.app_assoc.
 Qed.
 
-Lemma parse_member_name_complete sts pod ordinal :
-  pod.(PodV.ObjectMeta').(ObjectMetaV.Name') = desired_pod_name sts ordinal →
-  parse_member_name sts pod = Some ordinal.
+Lemma parse_member_name_complete set_name pod_name ordinal :
+  pod_name = desired_pod_name set_name ordinal →
+  parse_member_name set_name pod_name = Some ordinal.
 Proof.
   intros Hname.
   unfold parse_member_name.
@@ -105,12 +143,35 @@ Proof.
   apply parse_canonical_decimal_string_decimal_string.
 Qed.
 
-#[global] Instance pod_has_member_name_decision sts pod :
-  Decision (pod_has_member_name sts pod).
+#[global] Instance pod_has_member_name_decision set_name pod_name :
+  Decision (pod_has_member_name set_name pod_name).
 Proof.
-  destruct (parse_member_name sts pod) as [ordinal|] eqn:Hparse.
+  destruct (parse_member_name set_name pod_name) as [ordinal|] eqn:Hparse.
   - left. exists ordinal. by apply parse_member_name_sound.
   - right. intros [ordinal Hname].
+    apply parse_member_name_complete in Hname.
+    congruence.
+Defined.
+
+Definition pod_has_int32_member_name (set_name pod_name : go_string) : Prop :=
+  ∃ ordinal : nat,
+    (ordinal <= go_int32_max_nat)%nat ∧
+    pod_name = desired_pod_name set_name ordinal.
+
+#[global] Instance pod_has_int32_member_name_decision set_name pod_name :
+    Decision (pod_has_int32_member_name set_name pod_name).
+Proof.
+  unfold pod_has_int32_member_name.
+  destruct (parse_member_name set_name pod_name) as [ordinal|] eqn:Hparse.
+  - destruct (decide (ordinal <= go_int32_max_nat)%nat) as [Hbound|Hoverflow].
+    + left. exists ordinal. split; [done|].
+      by apply parse_member_name_sound.
+    + right. intros (ordinal' & Hbound & Hname).
+      apply parse_member_name_complete in Hname.
+      rewrite Hparse in Hname.
+      simplify_eq/=.
+      done.
+  - right. intros (ordinal & _ & Hname).
     apply parse_member_name_complete in Hname.
     congruence.
 Defined.
@@ -119,7 +180,9 @@ Lemma pod_has_member_key_iff sts pod :
   pod_has_member_key sts pod ↔
   pod.(PodV.ObjectMeta').(ObjectMetaV.Namespace') =
     sts.(StatefulSetV.ObjectMeta').(ObjectMetaV.Namespace') ∧
-  pod_has_member_name sts pod.
+  pod_has_member_name
+    sts.(StatefulSetV.ObjectMeta').(ObjectMetaV.Name')
+    pod.(PodV.ObjectMeta').(ObjectMetaV.Name').
 Proof.
   split.
   - intros [ordinal Hkey].
@@ -139,7 +202,9 @@ Proof.
   destruct (decide (
     pod.(PodV.ObjectMeta').(ObjectMetaV.Namespace') =
       sts.(StatefulSetV.ObjectMeta').(ObjectMetaV.Namespace') ∧
-    pod_has_member_name sts pod)) as [Hmember|Hnot_member].
+    pod_has_member_name
+      sts.(StatefulSetV.ObjectMeta').(ObjectMetaV.Name')
+      pod.(PodV.ObjectMeta').(ObjectMetaV.Name'))) as [Hmember|Hnot_member].
   - left. by apply pod_has_member_key_iff.
   - right. intros Hmember_key.
     apply Hnot_member. by apply pod_has_member_key_iff.
@@ -148,7 +213,9 @@ Defined.
 Example pod_has_member_name_accepts_one sts pod :
   pod.(PodV.ObjectMeta').(ObjectMetaV.Name') =
     sts.(StatefulSetV.ObjectMeta').(ObjectMetaV.Name') ++ "-1"%go →
-  pod_has_member_name sts pod.
+  pod_has_member_name
+    sts.(StatefulSetV.ObjectMeta').(ObjectMetaV.Name')
+    pod.(PodV.ObjectMeta').(ObjectMetaV.Name').
 Proof.
   intros Hname.
   exists 1%nat.
@@ -160,10 +227,14 @@ Qed.
 Example pod_has_member_name_rejects_leading_zero sts pod :
   pod.(PodV.ObjectMeta').(ObjectMetaV.Name') =
     sts.(StatefulSetV.ObjectMeta').(ObjectMetaV.Name') ++ "-01"%go →
-  ¬ pod_has_member_name sts pod.
+  ¬ pod_has_member_name
+    sts.(StatefulSetV.ObjectMeta').(ObjectMetaV.Name')
+    pod.(PodV.ObjectMeta').(ObjectMetaV.Name').
 Proof.
   intros Hname [ordinal Hmember].
-  pose proof (parse_member_name_complete sts pod ordinal Hmember) as Hparse.
+  pose proof (parse_member_name_complete
+    sts.(StatefulSetV.ObjectMeta').(ObjectMetaV.Name')
+    pod.(PodV.ObjectMeta').(ObjectMetaV.Name') ordinal Hmember) as Hparse.
   unfold parse_member_name, member_name_prefix in Hparse.
   rewrite Hname in Hparse.
   replace (sts.(StatefulSetV.ObjectMeta').(ObjectMetaV.Name') ++ "-01"%go)
